


\subsubsection{Mean Squared Error (MSE)}

% â€œImage2Mesh: A Learning Framework for Single Image 3D Reconstruction
% https://arxiv.org/abs/1711.10669
@misc{pontes2017image2mesh,
    title={Image2Mesh: A Learning Framework for Single Image 3D Reconstruction},
    author={Jhony K. Pontes and Chen Kong and Sridha Sridharan and Simon Lucey and Anders Eriksson and Clinton Fookes},
    year={2017},
    eprint={1711.10669},
    archivePrefix={arXiv},
    primaryClass={cs.CV}
}

This is defined as the surface distance between $X$ and $\hat{X}$:
\begin{align}
d(\hat{X},X) = \frac{1}{n_X} \sum_{p\in X}d(p,\hat{X})+\frac{1}{n_{\hat{X}}} \sum_{p\in \hat{X}}d(\hat{p},X).   
\end{align}
where ${n_X},n_{\hat{X}}$ as the number of sampled points, $p, \hat{p}$ are the point coordinates and $d(p,\hat{X}), d(\hat{p},X)$ are the distances along the normal direction to X, \textit{e.g} the $L_1, L_2$ norms:  
\begin{align}
x & = d(\hat{p},X) \\  
|x|_1 & = \Bigg[\sum_{k=1}^k|x_i|\Bigg|^1 \\  
|x|_2 & = \Bigg[\sum_{k=1}^k|x_k|^2\Bigg]^{\frac{1}{2}}  %
\end{align}

\subsubsection{Intersection over Union (IoU)}

%Stopped here, need to add this plus Mean of Cross Entropy loss 
%from
%https://arxiv.org/pdf/1906.06543.pdf

% Plus ideas, implementing on processor side (embedded CNN - tensorflow lite for Arduino) or on desktop side.
\begin{align}
IoU_{\epsilon} = \frac{\hat{V} \cap V} {\hat{V} \cup V} = \frac{\sum_i\{I(\hat{V_i}> \epsilon) * I(V_i)\}}{\sum_i\{I(I(\hat{V_i}> \epsilon) + I(V_i))\}}    
\end{align}

\subsubsection{Mean of Cross Entropy (CE) loss}

% source 3D Object Reconstruction from a Single Depth View with Adversarial Learning
% https://arxiv.org/abs/1708.07969
@misc{yang20173d,
    title={3D Object Reconstruction from a Single Depth View with Adversarial Learning},
    author={Bo Yang and Hongkai Wen and Sen Wang and Ronald Clark and Andrew Markham and Niki Trigoni},
    year={2017},
    eprint={1708.07969},
    archivePrefix={arXiv},
    primaryClass={cs.CV}
}

\begin{align}
CE = -\frac{1}{N}\sum_{i=1}^N\{p_ilog\hat{p}_i+(1-p_i)log(1 - \hat{p}_i)\} 
\end{align}